# Raw-Responses-of-NLP-Models_Mathematical_Logic
- Q1:***10+10=***
    - *ChatGPT:*
        >- The sum of 10 and 10 is 20.
        >- The sum of 10 and 10 is 20.
        >- The sum of 10 and 10 is 20.
    - *New Bing:*
        >- 10+10=20
        >- 20
        >- 10+10=20
    - *Wenxiyiyan:*
        >- 20
        >- 20
        >- 20
- Q2:***2+3+5+7+11+13+17+19+23+29+31+37+41+43+47+53+59+61+67+71=***
    - *ChatGPT:*
        >- The sum of the numbers you provided, from 2 to 71 (inclusive), is 958.
        >- The sum of the numbers you provided, from 2 to 71 (inclusive), is 831.
        >- The sum of the numbers you provided, 2 + 3 + 5 + 7 + 11 + 13 + 17 + 19 + 23 + 29 + 31 + 37 + 41 + 43 + 47 + 53 + 59 + 61 + 67 + 71, is 739.
    - *New Bing:*
        >- 639
        >- The sum of the prime numbers from 2 to 71 is 639.
        >- 2+3+5+7+11+13+17+19+23+29+31+37+41+43+47+53+59+61+67+71= 639
    - *Wenxinyiyan:*
        >- 2+3+5+7+11+13+17+19+23+29+31+37+41+43+47+53+59+61+67+71=639
        >- The result is 639
        >- 2+3+5+7+11+13+17+19+23+29+31+37+41+43+47+53+59+61+67+71=639
- Q3:***10X10-30=***
    - *ChatGPT:*
        >- The result of 10 multiplied by 10 minus 30 is 70.<br>
        To calculate it:<br>
        10 * 10 = 100<br>
        100 - 30 = 70
        >- 70
        >- 100-30=70
    - *New Bing:*
        >- 10*10-30=70
        >- 70
        >- 10×10−30=100-30=70
    - *Wenxinyiyan:*
        >- 10×10−30=70
        >- 10×10−30=70
        >- 70
- Q4:***x^2-2x+1=0***
    - *ChatGPT:*
        >- The equation x^2 - 2x + 1 = 0 is a quadratic equation. To solve it, we can use factoring or the quadratic formula.<br>
        Let's solve it by factoring:<br>
        x^2 - 2x + 1 = 0<br>
        The expression (x - 1)(x - 1) represents the factored form of the equation since (x - 1)^2 simplifies to x^2 - 2x + 1.<br>
        Now, to find the solution, we set each factor equal to zero:<br>
        x - 1 = 0<br>
        By adding 1 to both sides of the equation, we get:x = 1<br>
        Therefore, the solution to the equation x^2 - 2x + 1 = 0 is x = 1.
        >- The equation x^2 - 2x + 1 = 0 represents a quadratic equation. To solve it, we can use the fact that it can be factored as a perfect square:<br>
        x^2 - 2x + 1 = (x - 1)(x - 1)<br>
        Setting each factor equal to zero:<br>
        x - 1 = 0<br>
        Solving for x:<br>
        x = 1<br>
        Therefore, the solution to the equation x^2 - 2x + 1 = 0 is x = 1.
        >- The equation x^2 - 2x + 1 = 0 is a quadratic equation. To solve it, we can use the quadratic formula, which states that for an equation in the form ax^2 + bx + c = 0, the solutions for x are given by:<br>
        x = (-b ± √(b^2 - 4ac)) / (2a)<br>
        In this case, a = 1, b = -2, and c = 1. Substituting these values into the quadratic formula, we get:<br>
        x = (-(-2) ± √((-2)^2 - 4(1)(1))) / (2(1))<br>
          = (2 ± √(4 - 4)) / 2<br>
          = (2 ± √0) / 2<br>
          = (2 ± 0) / 2<br>
        The expression simplifies to:<br>
        x = 2 / 2 = 1<br>
        Therefore, the solution to the equation x^2 - 2x + 1 = 0 is x = 1.
    - *New Bing:*
        >- x^2-2x+1=0 is a quadratic equation that can be factored into (x-1)^2=0. The solution is x=1.
        >- The equation x^2-2x+1=0 is a quadratic equation. The roots of this equation are equal and are both 1. I hope that helps!
        >- x^2-2x+1=0 is a quadratic equation that can be factored as (x-1)^2=0. Therefore, the solution is x=1.
    - *Wenxinyiyan:*
        >- x=1
        >- x=1
        >- x=1
- Q5:***Coordinate of the intersection point of y=x and y=x^2***
    - *ChatGPT:*
        >- To find the coordinates of the intersection point between the two equations y = x and y = x^2, we can set them equal to each other:<br>
        x = x^2<br>
        Next, we rearrange the equation to bring all terms to one side:<br>
        x^2 - x = 0<br>
        Factoring out x, we have:<br>
        x(x - 1) = 0<br>
        From this equation, we can see that the solutions are x = 0 and x = 1.<br>
        To find the corresponding y-values, we substitute these x-values back into either of the original equations.<br>
        For x = 0:<br>
        y = 0<br>
        For x = 1:<br>
        y = 1^2 = 1<br>
        Therefore, the intersection points are (0, 0) and (1, 1).
        >- To find the coordinates of the intersection point between the two equations y = x and y = x^2, we can set them equal to each other:<br>
        x = x^2<br>
        By rearranging the equation, we get:<br>
        x^2 - x = 0<br>
        Factoring out x, we have:<br>
        x(x - 1) = 0<br>
        Setting each factor equal to zero, we get:<br>
        x = 0 or x - 1 = 0<br>
        From the first equation, x = 0.<br>
        From the second equation, x - 1 = 0, which gives x = 1.<br>
        Therefore, the two intersection points are (0, 0) and (1, 1).<br>
        >- To find the coordinates of the intersection point between the graphs of y = x and y = x^2, we can set the two equations equal to each other:<br>
        x = x^2<br>
        This equation can be rearranged as:<br>
        x^2 - x = 0<br>
        Factoring out x:<br>
        x(x - 1) = 0<br>
        Setting each factor equal to zero:<br>
        x = 0 or x - 1 = 0<br>
        Solving for x, we have two possible solutions:<br>
        x = 0 or x = 1<br>
        Substituting these values back into the equation y = x, we can find the corresponding y-coordinates:<br>
        For x = 0, y = 0<br>
        For x = 1, y = 1<br>
        Therefore, the intersection points are (0, 0) and (1, 1), where the graphs of y = x and y = x^2 intersect.
    - *New Bing:*
        >- The intersection point of y=x and y=x^2 is (0,0)
        >- The equation y=x and y=x^2 intersect at the point (0,0) and (1,1). I hope that helps!
        >- The intersection point of y=x and y=x^2 is (0,0) and (1,1).
    - *Wenxinyiyan:*
        >- The intersection point of y=x and y=x^2 is (1, 1).
        >- The intersection point of y=x and y=x^2 is (1,1).
        >- Solution: Find the intersection point of y=x and y=x^2<br>
        y=x and y=x^2 are equal, so we get x=x^2, which can be solved as x(1-x)=0. Therefore, two roots are x1=0 and x2=1.<br>
        The intersection points are (0,0) and (1,1).
